Revert "Keep track of a potentially erased fuel quantity."
This reverts commit 5bae408a6a0f0f90b2a900045abc2e7bd46d0c56.

pulse/lib/pulse/core/PulseCore.Action.fst
@@ -23,7 +23,6 @@ module Mem = PulseCore.MemoryAlt
 module I = PulseCore.InstantiatedSemantics
 module F = FStar.FunctionalExtensionality
 module ST = PulseCore.HoareStateMonad
-module PE = PulseCore.PotentiallyErased
 module Set = FStar.GhostSet
 friend PulseCore.InstantiatedSemantics
 
@@ -396,16 +395,23 @@ let later_elim (p:slprop)
 : act unit Ghost emp_inames (later p ** later_credit 1) (fun _ -> p)
 = fun #ictx -> ITA.later_elim ictx p
 
-let rec loop #t () : Dv t = loop ()
+let maybe_p (p:slprop) (b:erased bool) : slprop = if b then p else emp
+
+let maybe_buy
+: stt (erased bool) emp (maybe_p (later_credit 1))
+= stt_of_action0 (ITA.buy emp_inames)
+
+let rec reveal_div #t (b:erased bool) (k: squash (reveal b == true) -> t) : Dv t = 
+  reveal_div b k
 
 let buy1 ()
 : stt unit emp (fun _ -> later_credit 1)
 = I.bind 
-    (stt_of_action0 (ITA.buy emp_inames)) 
-    fun b -> I.hide_div fun _ -> 
-      PE.observe_bool b
-        (fun _ -> coerce_eq () <| I.return () fun _ -> later_credit 1)
-        (fun _ -> loop ())
+       maybe_buy 
+       (fun (b:erased bool) ->
+        I.hide_div (fun _ -> 
+          reveal_div b (fun _ -> 
+          coerce_eq () <| I.return () (fun _ -> later_credit 1))))
 
 ///////////////////////////////////////////////////////////////////
 // Core operations on references
