pulse/lib/pulse/core/PulseCore.InstantiatedSemantics.fst
@@ -32,12 +32,13 @@ let laws ()
 = Sep.sep_laws()
 
 let state0 (e:inames) : Sem.state u#4 = {
-    s = Sep.full_mem;
+    s = Sep.mem;
+    is_full_mem = Sep.is_full;
     pred = slprop;
     emp = emp;
     star = star;
-    interp = (fun p m -> interp p m.m);
-    invariant = (fun m -> mem_invariant e m.m);
+    interp;
+    invariant = mem_invariant e;
     laws = laws ();
 }
 
